@prefix xsd: <http://www.w3.org/2001/XMLSchema#> .
@prefix rdf: <http://www.w3.org/1999/02/22-rdf-syntax-ns#> .
@prefix rdfs: <http://www.w3.org/2000/01/rdf-schema#> .
@prefix owl: <http://www.w3.org/2002/07/owl#> .

@prefix dcterms: <http://purl.org/dc/terms/>.
@prefix skos: <http://www.w3.org/2004/02/skos/core#>.
@prefix foaf: <http://xmlns.com/foaf/0.1/>.
@prefix doap: <http://usefulinc.com/ns/doap#>.

@prefix vann: <http://purl.org/vocab/vann/>.

@prefix st: <http://purl.org/net/sparqltests/> .
@prefix ste: <http://purl.org/net/sparqltests/examples/> .


###
# classes
###

st:Test a owl:Class;
  rdfs:comment "A test description consists of a query string or a link to a query resource as well as an assertion. Optionally, success and fail messages can be added too." ;
  rdfs:label "SPARQL Query Test";
  dcterms:issued "2013-10-24"^^xsd:date ;
  dcterms:modified "2013-10-24"^^xsd:date ;
  rdfs:isDefinedBy <http://purl.org/net/sparqltests/> ;
  .

###
# properties
###

st:queryString a owl:DatatypeProperty;
  rdfs:comment "The string representation of the SPARQL query to executed for the test." ;
  rdfs:domain st:Test ;
  rdfs:label "query string" ;
  dcterms:issued "2013-10-23"^^xsd:date ;
  dcterms:modified "2013-10-24"^^xsd:date ;
  rdfs:isDefinedBy <http://purl.org/net/sparqltests/> ;
  .

st:successMessage a owl:DatatypeProperty;
  rdfs:comment "This message is used in the output or report if the query results fulfills the assertion." ;
  rdfs:domain st:Test ;
  rdfs:label "success message" ;
  dcterms:issued "2013-10-23"^^xsd:date ;
  dcterms:modified "2013-10-24"^^xsd:date ;
  rdfs:isDefinedBy <http://purl.org/net/sparqltests/> ;
  .

st:failMessage a owl:DatatypeProperty;
  rdfs:comment "This message is used in the output or report if the query result fulfills NOT the assertion." ;
  rdfs:domain st:Test ;
  rdfs:label "fail message" ;
  dcterms:issued "2013-10-23"^^xsd:date ;
  dcterms:modified "2013-10-24"^^xsd:date ;
  rdfs:isDefinedBy <http://purl.org/net/sparqltests/> ;
  .

st:skipMessage a owl:DatatypeProperty;
  rdfs:comment "This message is used in the output or report if the test is skipped because of a failed dependency." ;
  rdfs:domain st:Test ;
  rdfs:label "fail message" ;
  dcterms:issued "2013-10-23"^^xsd:date ;
  dcterms:modified "2013-10-24"^^xsd:date ;
  rdfs:isDefinedBy <http://purl.org/net/sparqltests/> ;
  .

st:depends a owl:ObjectProperty;
  rdfs:comment "Tests can depend on other tests. If one of the dependencies fail, the current test is skipped." ;
  rdfs:domain st:Test ;
  rdfs:range st:Test ;
  rdfs:label "depends" ;
  dcterms:issued "2013-10-23"^^xsd:date ;
  dcterms:modified "2013-10-24"^^xsd:date ;
  rdfs:isDefinedBy <http://purl.org/net/sparqltests/> ;
  .

st:assertEmpty a owl:DatatypeProperty;
  rdfs:domain st:Test ;
  rdfs:range xsd:boolean ;
  rdfs:comment "The empty assertion is true if the SPARQL result set is empty (no row)." ;
  rdfs:label "assert empty" ;
  dcterms:issued "2013-10-24"^^xsd:date ;
  dcterms:modified "2013-10-24"^^xsd:date ;
  rdfs:isDefinedBy <http://purl.org/net/sparqltests/> ;
  .

st:assertNotEmpty a owl:DatatypeProperty;
  rdfs:domain st:Test ;
  rdfs:range xsd:boolean ;
  rdfs:comment "The not empty assertion is true if the SPARQL result set has at least one solution (row)." ;
  rdfs:label "assert not empty" ;
  dcterms:issued "2013-10-24"^^xsd:date ;
  dcterms:modified "2013-10-24"^^xsd:date ;
  rdfs:isDefinedBy <http://purl.org/net/sparqltests/> ;
  .

###
# Example
###

ste:ExampleTestType a st:Test;
  rdfs:label "test for resources without rdf:type" ;
  st:queryString """SELECT ?s { ?s ?p ?o . OPTIONAL { ?s a ?type . } FILTER ( !bound(?type) ) . } LIMIT 1""" ;
  st:assertEmpty true ;
  st:failMessage "Some resources do not have an explizit rdf:type statement." ;
  dcterms:issued "2013-10-24"^^xsd:date ;
  dcterms:modified "2013-10-24"^^xsd:date ;
  rdfs:isDefinedBy <http://purl.org/net/sparqltests/> ;
  .

ste:ExampleTestMoreThanOneLable a st:Test;
  rdfs:label "test for resources with more than one rdf:label" ;
  st:queryString """SELECT ?s count(?label) { ?s rdfs:label ?label . } GROUP BY ?s HAVING (count(?label) > 1) LIMIT 1""";
  st:assertEmpty true ;
  st:failMessage "At least one resource has more than one rdfs:label values." ;
  dcterms:issued "2013-10-24"^^xsd:date ;
  dcterms:modified "2013-10-24"^^xsd:date ;
  rdfs:isDefinedBy <http://purl.org/net/sparqltests/> ;
  .

ste:ExampleTestMissingTranslation a st:Test;
  rdfs:label "test for missing german translation of english values" ;
  st:queryString """
SELECT ?valueen { ?s ?p ?valueen . FILTER ( lang(?valueen) = "en" )
OPTIONAL { ?s ?p ?valuede . FILTER ( lang(?valuede) = "de" ) }
FILTER ( !bound(?valuede) ) } LIMIT 1
""";
  st:assertEmpty true ;
  st:failMessage "At least one english literal has no german translation." ;
  dcterms:issued "2013-10-24"^^xsd:date ;
  dcterms:modified "2013-10-24"^^xsd:date ;
  rdfs:isDefinedBy <http://purl.org/net/sparqltests/> ;
  .

ste:ExampleTestValueMarkup a st:Test;
  rdfs:label "test for html tags in all literal values" ;
  st:queryString """SELECT ?markup { ?s ?property ?markup . FILTER isLiteral(?markup) . FILTER regex( ?markup, "<[a-z /]+>") . } LIMIT 1""";
  st:assertEmpty true ;
  st:failMessage "At least one literal value uses HTML markup." ;
  dcterms:issued "2013-10-24"^^xsd:date ;
  dcterms:modified "2013-10-24"^^xsd:date ;
  rdfs:isDefinedBy <http://purl.org/net/sparqltests/> ;
  .



###
# Vocabulary description and documentation
###

<http://purl.org/net/sparqltests/> a owl:Ontology;
    foaf:maker <http://sebastian.tramp.name>;
    doap:maintainer <http://sebastian.tramp.name>;
    vann:preferredNamespacePrefix "st";
    vann:preferredNamespaceUri "http://purl.org/net/sparqltest/";
    foaf:homepage <http://aksw.org/Projects/SparqlTests>;
    #vann:example <...>;
    #vann:changes <...>;
    rdfs:label "SPARQL Tests Description Vocabulary";
    dcterms:description "This is a simple and lightweight approach to provide a SPARQL query centered data test description framwork. ";
    dcterms:issued "2013-10-23"^^xsd:date ;
    dcterms:modified "2013-10-24"^^xsd:date ;
    rdfs:isDefinedBy <http://purl.org/net/sparqltests/> ;
    .

<http://sebastian.tramp.name> a foaf:Person; foaf:name "Sebastian Tramp".
