@prefix xsd: <http://www.w3.org/2001/XMLSchema#> .
@prefix rdfs: <http://www.w3.org/2000/01/rdf-schema#> .
@prefix owl: <http://www.w3.org/2002/07/owl#> .
@prefix dcterms: <http://purl.org/dc/terms/> .
@prefix foaf: <http://xmlns.com/foaf/0.1/> .
@prefix doap: <http://usefulinc.com/ns/doap#> .
@prefix vann: <http://purl.org/vocab/vann/> .
@prefix st: <http://purl.org/net/sparqltests/> .
@prefix ste: <http://purl.org/net/sparqltests/examples/> .

###
# Vocabulary description and documentation
###

<http://purl.org/net/sparqltests/> a owl:Ontology ;
  foaf:maker <http://sebastian.tramp.name> ;
  doap:maintainer <http://sebastian.tramp.name> ;
  vann:preferredNamespacePrefix "st" ;
  vann:preferredNamespaceUri "http://purl.org/net/sparqltest/" ;
  foaf:homepage <http://aksw.org/Projects/SparqlTests> ;
  #vann:changes <...> ;
  rdfs:label "SPARQL Tests Description Vocabulary" ;
  dcterms:description "This is a simple and lightweight approach to provide a SPARQL query centered data test description framework." ;
  dcterms:issued "2013-10-23"^^xsd:date ;
  dcterms:modified "2013-10-24"^^xsd:date ;
  rdfs:isDefinedBy <http://purl.org/net/sparqltests/> ;
  .

###
# classes
###

st:Test a owl:Class ;
  rdfs:comment "A test description consists of a query string as well as an result assertion. Optionally, success, fail and skip messages can be added." ;
  rdfs:label "SPARQL Test" ;
  dcterms:issued "2013-10-24"^^xsd:date ;
  dcterms:modified "2013-10-24"^^xsd:date ;
  rdfs:isDefinedBy <http://purl.org/net/sparqltests/> ;
  vann:example ste:TestFoafPerson, ste:TestFoafPersonMissingValues, ste:TestMissingPropertyDescription,
    ste:TestMissingClassDescription, ste:TestMissingTranslation, ste:TestMoreThanOneLabel,
    ste:TestMoreThanOneLabel, ste:TestType, ste:TestValueMarkup, ste:TestWrongObjectPropertyValues ;
  .

###
# properties
###

st:queryString a owl:DatatypeProperty ;
  rdfs:comment "The string representation of the SPARQL query to executed for the test." ;
  rdfs:domain st:Test ;
  rdfs:label "query string" ;
  dcterms:issued "2013-10-23"^^xsd:date ;
  dcterms:modified "2013-10-24"^^xsd:date ;
  rdfs:isDefinedBy <http://purl.org/net/sparqltests/> ;
  .

st:successMessage a owl:DatatypeProperty ;
  rdfs:comment "This message is used in the output or report if the test successes." ;
  rdfs:domain st:Test ;
  rdfs:label "success message" ;
  dcterms:issued "2013-10-23"^^xsd:date ;
  dcterms:modified "2013-10-24"^^xsd:date ;
  rdfs:isDefinedBy <http://purl.org/net/sparqltests/> ;
  .

st:failMessage a owl:DatatypeProperty ;
  rdfs:comment "This message is used in the output or report if the test fails." ;
  rdfs:domain st:Test ;
  rdfs:label "fail message" ;
  dcterms:issued "2013-10-23"^^xsd:date ;
  dcterms:modified "2013-10-24"^^xsd:date ;
  rdfs:isDefinedBy <http://purl.org/net/sparqltests/> ;
  .

st:skipMessage a owl:DatatypeProperty;
  rdfs:comment "This message is used in the output or report if the test was skipped because of a failed dependency." ;
  rdfs:domain st:Test ;
  rdfs:label "fail message" ;
  dcterms:issued "2013-10-23"^^xsd:date ;
  dcterms:modified "2013-10-24"^^xsd:date ;
  rdfs:isDefinedBy <http://purl.org/net/sparqltests/> ;
  .

st:depends a owl:ObjectProperty;
  rdfs:comment "Tests can depend on other tests. If one of the dependencies fail, the current test is skipped." ;
  rdfs:domain st:Test ;
  rdfs:range st:Test ;
  rdfs:label "depends" ;
  dcterms:issued "2013-10-23"^^xsd:date ;
  dcterms:modified "2013-10-24"^^xsd:date ;
  rdfs:isDefinedBy <http://purl.org/net/sparqltests/> ;
  .

st:assertEmpty a owl:DatatypeProperty;
  rdfs:domain st:Test ;
  rdfs:range xsd:boolean ;
  rdfs:comment "The empty assertion is true if the SPARQL result set is empty (no row)." ;
  rdfs:label "assert empty" ;
  dcterms:issued "2013-10-24"^^xsd:date ;
  dcterms:modified "2013-10-24"^^xsd:date ;
  rdfs:isDefinedBy <http://purl.org/net/sparqltests/> ;
  .

st:assertNotEmpty a owl:DatatypeProperty;
  rdfs:domain st:Test ;
  rdfs:range xsd:boolean ;
  rdfs:comment "The not empty assertion is true if the SPARQL result set has at least one solution (row)." ;
  rdfs:label "assert not empty" ;
  dcterms:issued "2013-10-24"^^xsd:date ;
  dcterms:modified "2013-10-24"^^xsd:date ;
  rdfs:isDefinedBy <http://purl.org/net/sparqltests/> ;
  .

###
# Example
###
ste:TestMissingClassDescription a st:Test;
  rdfs:label "test for missing class descriptions of used classes" ;
  st:queryString """
SELECT DISTINCT ?class {
  ?subject a ?class .
  OPTIONAL { ?class ?classProperty ?classValue . }
  FILTER ( !bound(?classValue) )
} LIMIT 1
""" ;
  st:assertEmpty true ;
  st:failMessage "Some classes are used but do not have a description." ;
  dcterms:issued "2013-10-24"^^xsd:date ;
  dcterms:modified "2013-10-24"^^xsd:date ;
  rdfs:isDefinedBy <http://purl.org/net/sparqltests/> ;
  .

ste:TestMissingPropertyDescription a st:Test;
  rdfs:label "test for missing property descriptions of used properties" ;
  st:queryString """
SELECT DISTINCT ?property {
  ?subject ?property ?value .
  OPTIONAL { ?property ?propertyProperty ?propertyValue . }
  FILTER ( !bound(?propertyValue) )
} LIMIT 1
""" ;
  st:assertEmpty true ;
  st:failMessage "Some properties are used but do not have a description." ;
  dcterms:issued "2013-10-24"^^xsd:date ;
  dcterms:modified "2013-10-24"^^xsd:date ;
  rdfs:isDefinedBy <http://purl.org/net/sparqltests/> ;
  .


ste:TestType a st:Test;
  rdfs:label "test for resources without rdf:type" ;
  st:queryString """
SELECT ?s {
  ?s ?p ?o .
  OPTIONAL { ?s a ?type . }
  FILTER ( !bound(?type) ) .
} LIMIT 1
""" ;
  st:assertEmpty true ;
  st:failMessage "Some resources do not have an explizit rdf:type statement." ;
  dcterms:issued "2013-10-24"^^xsd:date ;
  dcterms:modified "2013-10-24"^^xsd:date ;
  rdfs:isDefinedBy <http://purl.org/net/sparqltests/> ;
  .

ste:TestMoreThanOneLabel a st:Test;
  rdfs:label "test for resources with more than one rdf:label value" ;
  st:queryString """
SELECT ?s count(?label) {
  ?s rdfs:label ?label .
} GROUP BY ?s HAVING (count(?label) > 1)
LIMIT 1
""";
  st:assertEmpty true ;
  st:failMessage "At least one resource has more than one rdfs:label values." ;
  dcterms:issued "2013-10-24"^^xsd:date ;
  dcterms:modified "2013-10-24"^^xsd:date ;
  rdfs:isDefinedBy <http://purl.org/net/sparqltests/> ;
  .

ste:TestMissingTranslation a st:Test;
  rdfs:label "test for missing german translation of english values" ;
  st:queryString """
SELECT ?subject ?property ?valueen {
  ?subject ?property ?valueen .
  FILTER ( lang(?valueen) = "en" )
  OPTIONAL {
    ?subject ?property ?valuede .
    FILTER ( lang(?valuede) = "de" )
  }
  FILTER ( !bound(?valuede) )
} LIMIT 1
""";
  st:assertEmpty true ;
  st:failMessage "At least one english literal has no german translation." ;
  dcterms:issued "2013-10-24"^^xsd:date ;
  dcterms:modified "2013-10-24"^^xsd:date ;
  rdfs:isDefinedBy <http://purl.org/net/sparqltests/> ;
  .

ste:TestValueMarkup a st:Test;
  rdfs:label "test for html tags in all literal values" ;
  st:queryString """
SELECT ?s ?property ?markup {
  ?s ?property ?markup .
  FILTER isLiteral(?markup) .
  FILTER regex( ?markup, "<[a-z /]+>") .
} LIMIT 1
""";
  st:assertEmpty true ;
  st:failMessage "At least one literal value uses HTML markup." ;
  dcterms:issued "2013-10-24"^^xsd:date ;
  dcterms:modified "2013-10-24"^^xsd:date ;
  rdfs:isDefinedBy <http://purl.org/net/sparqltests/> ;
  .

ste:TestFoafPerson a st:Test;
  rdfs:label "dependency test for foaf:Person tests" ;
  st:queryString """
PREFIX foaf: <http://xmlns.com/foaf/0.1/>
SELECT ?person {
  ?person a foaf:Person
} LIMIT 1
""";
  st:assertNotEmpty true ;
  st:successMessage "Found foaf:Person resources." ;
  dcterms:issued "2013-10-24"^^xsd:date ;
  dcterms:modified "2013-10-24"^^xsd:date ;
  rdfs:isDefinedBy <http://purl.org/net/sparqltests/> ;
  .

ste:TestFoafPersonMissingValues a st:Test ;
  rdfs:label "tests foaf:Person resources for specific attributes" ;
  st:depends ste:TestFoafPerson ;
  st:queryString """
PREFIX foaf: <http://xmlns.com/foaf/0.1/>
SELECT * {
  ?person a foaf:Person .
  OPTIONAL { ?person foaf:firstName ?firstName }
  OPTIONAL { ?person foaf:lastName ?lastName }
  OPTIONAL { ?person foaf:depiction ?depiction }
  FILTER (
    !bound(?firstName) ||
    !bound(?lastName) ||
    !bound(?depiction)
  )
} LIMIT 1
""" ;
  st:assertEmpty true ;
  st:failMessage "foaf:Person resources need at least firstName, lastName and depiction" ;
  dcterms:issued "2013-10-24"^^xsd:date ;
  dcterms:modified "2013-10-24"^^xsd:date ;
  rdfs:isDefinedBy <http://purl.org/net/sparqltests/> ;
  .

ste:TestWrongObjectPropertyValues a st:Test ;
  rdfs:label "tests of wrong" ;
  st:queryString """
SELECT * {
  ?property a owl:ObjectProperty .
  ?subject ?property ?value.
  FILTER (!isUri(?value))
} LIMIT 1
""" ;
  st:assertEmpty true ;
  st:failMessage "Some values of owl:ObjectProperties are not resources (but Literals)" ;
  dcterms:issued "2013-10-24"^^xsd:date ;
  dcterms:modified "2013-10-24"^^xsd:date ;
  rdfs:isDefinedBy <http://purl.org/net/sparqltests/> ;
  .


###
# misc resources
###

<http://sebastian.tramp.name> a foaf:Person; foaf:name "Sebastian Tramp".
